Robots

doc/tutorial/code/solutions_universes/Ex11a.fst
@@ -1,9 +1,22 @@
 module Ex11a
 
 open FStar.Heap
-open FStar.Util
 open FStar.HyperHeap
+open FStar.Set
 
+let only (#t:eqtype) (i:t) =
+  singleton i
+
+let op_Hat_Plus_Hat (r1:rid) (r2:rid) =
+  union (singleton r1) (singleton r2)
+
+let op_Plus_Plus_Hat (s:set rid) (r2:rid) =
+  union s (singleton r2)
+
+type distinct (r:rid) (s:set rid) =
+  forall x. Set.mem x s ==> disjoint x r
+
+// BEGIN: Types
 type point =
   | Point : #r:rid
           -> x:rref r int
@@ -26,7 +39,9 @@ type bot =
                       /\ disjoint (Point.r pos) (Arm.r right)
                       /\ disjoint (Arm.r left)  (Arm.r right)}
         -> bot
+// END: Types
 
+// BEGIN: Invariant
 let flying (b:bot) (h:HyperHeap.t) =
   sel h (Point.z (Bot.pos b)) > 0
 
@@ -40,67 +55,18 @@ type robot_inv (b:bot) (h:HyperHeap.t) =
   /\ Map.contains h (Arm.r (Bot.left b))
   /\ Map.contains h (Arm.r (Bot.right b))
   /\ (flying b h ==> arms_up b h)
+// END: Invariant
 
-let only i = Set.singleton i
-
-val fly: b:bot -> ST unit
-  (requires (robot_inv b))
-  (ensures (fun h0 _u h1 ->
-                modifies (only (Bot.r b)) h0 h1
-              /\ robot_inv b h1
-              /\ flying b h1))
-let fly b =
-  Arm.azim (Bot.right b)  := 17;
-  Arm.polar (Bot.left b)  := 0;
-  Arm.polar (Bot.right b) := 0;
-  Point.z (Bot.pos b)     := 100
-
-val fly_robots: b0:bot -> b1:bot{disjoint (Bot.r b0) (Bot.r b1)}
-  -> ST unit
-    (requires (fun h -> robot_inv b0 h /\ robot_inv b1 h))
-    (ensures (fun h0 x h1 ->
-                modifies (Bot.r b0 ^+^ Bot.r b1) h0 h1
-              /\ robot_inv b0 h1
-              /\ robot_inv b1 h1
-              /\ flying b0 h1
-              /\ flying b1 h1))
-let fly_robots b0 b1 =
-  fly b0;
-  fly b1
-
-val fly_one: b0:bot -> b1:bot{disjoint (Bot.r b0) (Bot.r b1)}
-  -> ST unit
-    (requires (fun h -> robot_inv b0 h /\ robot_inv b1 h /\ ~(flying b1 h)))
-    (ensures (fun h0 x h1 ->
-                modifies (Bot.r b0 ^+^ Bot.r b1) h0 h1
-              /\ robot_inv b0 h1
-              /\ robot_inv b1 h1
-              /\ flying b0 h1
-              /\ ~(flying b1 h1)))
-let fly_one b0 b1 =
-  fly b0
-
-val lemma_frame_robot_inv1 : b:bot -> h0:HyperHeap.t -> h1:HyperHeap.t -> i:rid{disjoint i (Bot.r b)}
-  -> Lemma (requires (robot_inv b h0 /\ modifies (only i) h0 h1))
-           (ensures (robot_inv b h1))
-let lemma_frame_robot_inv1 b h0 h1 i = ()
-
-val lemma_frame_robot_inv2 : b:bot -> h0:HyperHeap.t -> h1:HyperHeap.t -> s:Set.set rid
-  -> Lemma (requires (robot_inv b h0
-                     /\ modifies s h0 h1
-                     /\ (forall r. Set.mem r s ==> disjoint r (Bot.r b))))
-           (ensures (robot_inv b h1))
-let lemma_frame_robot_inv2 b h0 h1 s = ()
-
+// BEGIN: Build
 val new_point: r0:rid -> x:int -> y:int -> z:int -> ST point
-    (requires (fun h0 -> True))
-    (ensures (fun h0 p h1 ->
-          modifies Set.empty h0 h1
-          /\ extends (Point.r p) r0
-          /\ fresh_region (Point.r p) h0 h1
-          /\ sel h1 (Point.x p) = x
-          /\ sel h1 (Point.y p) = y
-          /\ sel h1 (Point.z p) = z))
+  (requires (fun h0 -> True))
+  (ensures (fun h0 p h1 ->
+              modifies empty h0 h1
+            /\ extends (Point.r p) r0
+            /\ fresh_region (Point.r p) h0 h1
+            /\ sel h1 (Point.x p) = x
+            /\ sel h1 (Point.y p) = y
+            /\ sel h1 (Point.z p) = z))
 let new_point r0 x y z =
   let r = new_region r0 in
   let x = ralloc r x in
@@ -109,109 +75,121 @@ let new_point r0 x y z =
   Point x y z
 
 val new_arm: r0:rid -> ST arm
-    (requires (fun h0 -> True))
-    (ensures (fun h0 x h1 ->
-          modifies Set.empty h0 h1
-          /\ extends (Arm.r x) r0
-          /\ fresh_region (Arm.r x) h0 h1))
+  (requires (fun h0 -> True))
+  (ensures (fun h0 x h1 ->
+              modifies empty h0 h1
+            /\ extends (Arm.r x) r0
+            /\ fresh_region (Arm.r x) h0 h1))
 let new_arm r0 =
   let r = new_region r0 in
   let p = ralloc r 0 in
   let a = ralloc r 0 in
   Arm p a
 
-val test: r0:rid -> ST unit (requires (fun _ -> True)) (ensures (fun _ _ _ -> True))
-let test r0 =
-  let r = new_region r0 in
-  let m0 = get() in
-  cut (b2t(Map.contains m0 r));
-  let m1 = magic() in
-  admitP (modifies Set.empty m0 m1);
-  assert (Map.contains m1 r)
-
-val test1: r0:rid -> ST unit (requires (fun m0 -> Map.contains m0 r0)) (ensures (fun _ _ _ -> True))
-let test1 r0 =
-  let x = ralloc r0 0 in
-  let m0 = get() in
-  assert (sel m0 x = 0);
-  let m1 = magic() in
-  admitP (modifies Set.empty m0 m1);
-  assert (sel m1 x = 0)
-
-val new_robot: r0:rid -> ST bot (requires (fun h0 -> True))
-                                (ensures (fun h0 x h1 ->
-                                      modifies Set.empty h0 h1
-                                      /\ extends (Bot.r x) r0
-                                      /\ fresh_region (Bot.r x) h0 h1
-                                      /\ robot_inv x h1))
+val new_robot: r0:rid -> ST bot
+  (requires (fun h0 -> True))
+  (ensures (fun h0 x h1 ->
+	      modifies empty h0 h1
+            /\ extends (Bot.r x) r0
+            /\ fresh_region (Bot.r x) h0 h1
+            /\ robot_inv x h1))
 let new_robot r0 =
   let r = new_region r0 in
   let p = new_point r 0 0 0 in
   let left = new_arm r in
   let right = new_arm r in
   Bot #r p left right
+// END: Build
 
 val walk_robot_to: x:int -> y:int -> b:bot -> ST unit
-    (requires (robot_inv b))
-    (ensures (fun h0 u h1 ->
-                modifies (only (Point.r (Bot.pos b))) h0 h1
-                /\ robot_inv b h1
-                /\ sel h1 (Point.z (Bot.pos b))  = sel h1 (Point.z (Bot.pos b))
-                /\ sel h1 (Point.x (Bot.pos b))  = x
-                /\ sel h1 (Point.y (Bot.pos b))  = y))
+  (requires (robot_inv b))
+  (ensures (fun h0 u h1 ->
+              modifies (only (Point.r (Bot.pos b))) h0 h1
+            /\ robot_inv b h1
+            /\ sel h1 (Point.z (Bot.pos b)) = sel h1 (Point.z (Bot.pos b))
+            /\ sel h1 (Point.x (Bot.pos b)) = x
+            /\ sel h1 (Point.y (Bot.pos b)) = y))
 let walk_robot_to x y b =
   Point.x (Bot.pos b) := x;
   Point.y (Bot.pos b) := y
 
+// BEGIN: Fly
+val fly: b:bot -> ST unit
+  (requires (fun h -> robot_inv b h))
+  (ensures (fun h0 _u h1 ->
+              modifies (only (Bot.r b)) h0 h1
+            /\ robot_inv b h1
+            /\ flying b h1))
+let fly b =
+  Arm.azim (Bot.right b)  := 17;
+  Arm.polar (Bot.left b)  := 0;
+  Arm.polar (Bot.right b) := 0;
+  Point.z (Bot.pos b)     := 100
+// END: Fly
 
-open FStar.Set
+// BEGIN: FlyBoth
+val fly_both: b0:bot -> b1:bot{disjoint (Bot.r b0) (Bot.r b1)}
+  -> ST unit
+  (requires (fun h -> robot_inv b0 h /\ robot_inv b1 h))
+  (ensures (fun h0 x h1 ->
+              modifies (Bot.r b0 ^+^ Bot.r b1) h0 h1
+            /\ robot_inv b0 h1
+            /\ robot_inv b1 h1
+            /\ flying b0 h1
+            /\ flying b1 h1))
+let fly_both b0 b1 =
+  fly b0;
+  fly b1
+// END: FlyBoth
 
-type distinct (r:rid) (s:set rid) =
-  forall x. Set.mem x s ==> disjoint x r
+val fly_one: b0:bot -> b1:bot{disjoint (Bot.r b0) (Bot.r b1)} -> ST unit
+  (requires (fun h -> robot_inv b0 h /\ robot_inv b1 h /\ ~(flying b1 h)))
+  (ensures (fun h0 x h1 ->
+              modifies (only (Bot.r b0)) h0 h1
+            /\ robot_inv b0 h1
+            /\ robot_inv b1 h1
+            /\ flying b0 h1
+            /\ ~(flying b1 h1)))
+let fly_one b0 b1 =
+  fly b0
 
-#set-options "--initial_fuel 2 --max_fuel 2 --initial_ifuel 1 --max_ifuel 1"
-type bots : set rid -> Type =
-  | Nil    : bots Set.empty
-  | Cons   :  #rs:set rid
-           -> hd:bot{distinct (Bot.r hd) rs}
-           -> tl:bots rs
-           -> bots (rs ++^ Bot.r hd)
+noeq type bots : set rid -> Type =
+  | Nil : bots empty
+  | Cons : #rs:set rid
+         -> hd:bot{distinct (Bot.r hd) rs}
+         -> tl:bots rs
+         -> bots (rs ++^ Bot.r hd)
+
 val mem : #rs:set rid -> bot -> bs:bots rs -> Tot bool (decreases bs)
-let rec mem  (#rs:set rid) b bs = match bs with
+let rec mem  (#rs:set rid) b = function
   | Nil -> false
-  | Cons hd tl -> b=hd || mem b tl
+  | Cons hd tl -> b = hd || mem b tl
 
-val lemma_aux: #rs:set rid -> bs:bots rs -> b:bot
-             -> Lemma (requires (mem #rs b bs))
-                      (ensures (Set.mem (Bot.r b) rs))
-                      (decreases bs)
-                      [SMTPat (mem #rs b bs)]
-let rec lemma_aux #rs bs b =
+val lemma_mem_rid: #rs:set rid -> bs:bots rs -> b:bot
+  -> Lemma (requires (mem #rs b bs))
+          (ensures (Set.mem (Bot.r b) rs))
+	  (decreases bs)
+          [SMTPat (mem #rs b bs)]
+let rec lemma_mem_rid #rs bs b =
   match bs with
-    | Nil -> ()
-    | Cons hd tl ->
-      if b=hd
-      then ()
-      else lemma_aux tl b
+  | Nil -> ()
+  | Cons hd tl -> if b <> hd then lemma_mem_rid tl b
 
-val lemma_bots_tl_disjoint : #rs:set rid -> bs:bots rs{is_Cons bs}
-                           -> Lemma (requires (True))
-                                    (ensures (forall b. mem b (Cons.tl bs) ==> disjoint (Bot.r b) (Bot.r (Cons.hd bs))))
+val lemma_bots_tl_disjoint: #rs:set rid -> bs:bots rs{is_Cons bs}
+  -> Lemma (requires True)
+          (ensures (forall b. let Cons hd tl = bs in
+			 mem b tl ==> disjoint (Bot.r b) (Bot.r hd)))
 let lemma_bots_tl_disjoint #rs bs = ()
 
-(* remove the assume and implement this function *)
-assume val fly_robot_army:  #rs:Set.set rid
-                  -> bs:bots rs
-                  -> ST unit
-                     (requires (fun h -> (forall b. mem b bs ==> robot_inv b h)))
-                     (ensures  (fun h0 _u h1 ->
-                                    modifies rs h0 h1
-                                     /\ (forall b. mem b bs ==> robot_inv b h1 /\ flying b h1)))
-
-val main: unit -> ST unit
-    (requires (fun _ -> True))
-    (ensures (fun m0 _ m1 -> modifies Set.empty m0 m1))
-let main () =
-  let b1 = new_robot root in
-  let b2 = new_robot root in
-  fly_robots b1 b2
+val fly_robot_army: #rs:set rid -> bs:bots rs -> ST unit
+  (requires (fun h -> (forall b. mem b bs ==> robot_inv b h)))
+  (ensures  (fun h0 _u h1 ->   modifies rs h0 h1
+                          /\ (forall b. mem b bs ==> robot_inv b h1 /\ flying b h1)))
+let rec fly_robot_army #rs bs =
+  match bs with
+  | Nil -> ()
+  | Cons #rs' b bs' ->
+    //cut (rs == (rs' ++^ Bot.r b));  //not necesary, doesn't improve speed
+    //lemma_bots_tl_disjoint bs;      //not necessary; doesnt' improve speed
+    fly b;
+    fly_robot_army bs'
